Risolvere la seguente disequazione $\dfrac{x^2-2x+3}{3+5x-3x^2}\geq 0$
\begin{align*}
3+5x-3x^2>&0\\
3+5x-3x^2=&0\\
x_{1,2}=&\xunodue{-3}{5}{+3}=\dfrac{-5\pm\sqrt{25+24}}{-6}\\
=&\dfrac{-5\pm\sqrt{49}}{-6}\\
=&\dfrac{-5\pm 7}{12}=\begin{cases}
x_1=\dfrac{-12}{-6}=2\\
x_2=\dfrac{1}{-6}=-\dfrac{1}{6}
\end{cases}\\
x^2-2x+3\geq&0\\
x^2-2x+3=&0\\
x_{1,2}=&\xunodue{1}{-2}{+3}=\dfrac{2\pm\sqrt{4-12}}{2}\\
=&\dfrac{2\pm\sqrt{-8}}{2}
\qquad\text{nessuna soluzione}\\
\end{align*}
\begin{center}
	\includestandalone{grafici/disfrazFA1}
\end{center}
La frazione Ã¨ positiva ma non nulla per
\begin{align*}
-\dfrac{1}{6}<&x<2\\
\end{align*}
