	Risolvere la seguente disequazione $\dfrac{3x^2+x-2}{5+4x^2-3x}\leq 0$
	\begin{align*}
	5+4x^2-3x>&0\\
5+4x^2-3x=&0\\
x_{1,2}=&\xunodue{4}{-3}{5}=\dfrac{3\pm\sqrt{9-80}}{8}\\
=&\dfrac{3\pm\sqrt{-71}}{8}
\qquad\text{nessuna soluzione}\\
3x^2+x-2>&0\\
3x^2+x-2=&0\\
x_{1,2}=&\xunodue{3}{+1}{-2}=\dfrac{-1\pm\sqrt{1+24}}{6}\\
=&\dfrac{-1\pm\sqrt{25}}{6}\\
=&\dfrac{-1\pm 5}{6}=\begin{cases}
x_1=\dfrac{6}{6}=1\\
x_2=\dfrac{-4}{6}=-\dfrac{2}{3}
\end{cases}\\
	\end{align*}
	\begin{center}
		\includestandalone{grafici/disfrazCA2}
	\end{center}
assume valori negativi ed uguale a zero per:
\begin{align*}
-\dfrac{2}{3}\leq&x\leq 1\\
\end{align*}
