	Risolvere la seguente disequazione $\dfrac{1-6x^2-3x}{-x^2-6x-9}\geq 0$
	\begin{align*}
	-x^2-6x-9>&0\\
	-x^2-6x-9=&0\\
	x_{1,2}=&\xunodue{-1}{-6}{7}=\dfrac{6\pm\sqrt{36-36}}{-2}\\
	=&\dfrac{6\pm\sqrt{0}}{-2}=\dfrac{6}{-2}=-3\\
	1-6x^2-3x>&0\\
	1-6x^2-3x=&0\\
	x_{1,2}=&\xunodue{-6}{-3}{1}=\dfrac{1\pm\sqrt{1+24}}{-12}\\
	=&\dfrac{1\pm\sqrt{25}}{-12}=\dfrac{1\pm 5}{-12}=\begin{cases}
	x_1=\dfrac{6}{-12}=-\dfrac{1}{2}\\
	x_2=\dfrac{-4}{-12}=\dfrac{1}{3}
	\end{cases}\\
	\end{align*}
	\begin{center}
		\includestandalone{grafici/disfrazDE1}
	\end{center}
La frazione Ã¨ positiva per
	\begin{align*}
	x<&-3\\ -3<&x<-\dfrac{1}{2}\\ \dfrac{1}{3}\leq x\\
	\end{align*}
